Extract val_rel to separate file

theories/simplang/heapbij.v
@@ -5,7 +5,7 @@ From simuliris.base_logic Require Export gen_sim_heap gen_sim_prog.
 From simuliris.simulation Require Import slsls lifting.
 From iris.algebra.lib Require Import gset_bij.
 From iris.base_logic.lib Require Import gset_bij.
-From simuliris.simplang Require Export class_instances primitive_laws.
+From simuliris.simplang Require Export class_instances primitive_laws val_rel.
 
 From iris.prelude Require Import options.
 
@@ -38,6 +38,7 @@ End definitions.
 Notation "b_t '⇔h' b_s" := (heap_bij_elem b_t b_s) (at level 30) : bi_scope.
 Definition loc_rel `{heapbijG Σ} l_t l_s : iProp Σ := loc_chunk l_t ⇔h loc_chunk l_s ∗ ⌜loc_idx l_t = loc_idx l_s⌝.
 Notation "l_t '↔h' l_s" := (loc_rel l_t l_s) (at level 30) : bi_scope.
+Definition val_rel `{heapbijG Σ} := struct_val_rel loc_rel.
 
 Section laws.
   Context `{heapbijG Σ}.
@@ -90,157 +91,42 @@ Section laws.
     iIntros "[Hi %Hj]". iSplitL "Hi"; first done. iPureIntro.
     destruct l_t, l_s; cbn in *; lia.
   Qed.
+
+  Lemma val_rel_func v1 v2 v3 : val_rel v1 v2 -∗ val_rel v1 v3 -∗ ⌜v2 = v3⌝.
+  Proof.
+    iIntros "Hv1 Hv2". iInduction v2 as [[n2 | b2 | | | l2 | f2 ] | v2_1 v2_2 | v2 | v2] "IH" forall (v1 v3); val_discr_source "Hv1"; val_discr_target "Hv2"; try done.
+    - iPoseProof (struct_val_rel_loc_source with "Hv1") as (?) "(-> & Hl1)".
+      iPoseProof (struct_val_rel_loc_target with "Hv2") as (?) "(-> & Hl2)".
+      by iPoseProof (heap_bij_loc_func with "Hl1 Hl2") as "->".
+    - iPoseProof (struct_val_rel_pair_source with "Hv1") as (??) "(-> & Hv1_1 & Hv1_2)".
+      iPoseProof (struct_val_rel_pair_target with "Hv2") as (??) "(-> & Hv2_1 & Hv2_2)".
+      iPoseProof ("IH" with "Hv1_1 Hv2_1") as "->".
+      by iPoseProof ("IH1" with "Hv1_2 Hv2_2") as "->".
+    - iPoseProof (struct_val_rel_injl_source with "Hv1") as (?) "(-> & Hv1)".
+      iPoseProof (struct_val_rel_injl_target with "Hv2") as (?) "(-> & Hv2)".
+      by iPoseProof ("IH" with "Hv1 Hv2") as "->".
+    - iPoseProof (struct_val_rel_injr_source with "Hv1") as (?) "(-> & Hv1)".
+      iPoseProof (struct_val_rel_injr_target with "Hv2") as (?) "(-> & Hv2)".
+      by iPoseProof ("IH" with "Hv1 Hv2") as "->".
+  Qed.
+  Lemma val_rel_inj v1 v2 v3 : val_rel v2 v1 -∗ val_rel v3 v1 -∗ ⌜v2 = v3⌝.
+  Proof.
+    iIntros "Hv1 Hv2". iInduction v2 as [[n2 | b2 | | | l2 | f2 ] | v2_1 v2_2 | v2 | v2] "IH" forall (v1 v3); val_discr_target "Hv1"; val_discr_source "Hv2"; try done.
+    - iPoseProof (struct_val_rel_loc_target with "Hv1") as (?) "(-> & Hl1)".
+      iPoseProof (struct_val_rel_loc_source with "Hv2") as (?) "(-> & Hl2)".
+      by iPoseProof (heap_bij_loc_inj with "Hl1 Hl2") as "->".
+    - iPoseProof (struct_val_rel_pair_target with "Hv1") as (??) "(-> & Hv1_1 & Hv1_2)".
+      iPoseProof (struct_val_rel_pair_source with "Hv2") as (??) "(-> & Hv2_1 & Hv2_2)".
+      iPoseProof ("IH" with "Hv1_1 Hv2_1") as "->".
+      by iPoseProof ("IH1" with "Hv1_2 Hv2_2") as "->".
+    - iPoseProof (struct_val_rel_injl_target with "Hv1") as (?) "(-> & Hv1)".
+      iPoseProof (struct_val_rel_injl_source with "Hv2") as (?) "(-> & Hv2)".
+      by iPoseProof ("IH" with "Hv1 Hv2") as "->".
+    - iPoseProof (struct_val_rel_injr_target with "Hv1") as (?) "(-> & Hv1)".
+      iPoseProof (struct_val_rel_injr_source with "Hv2") as (?) "(-> & Hv2)".
+      by iPoseProof ("IH" with "Hv1 Hv2") as "->".
+  Qed.
 End laws.
-
-(** ** Default value relation *)
-Section val_rel.
-  Context `{heapbijG Σ}.
-  Fixpoint val_rel (v_t v_s : val) {struct v_s} : iProp Σ :=
-    match v_t, v_s with
-    | LitV (LitLoc l_t), LitV (LitLoc l_s) =>
-        l_t ↔h l_s
-    | LitV l_t, LitV l_s =>
-        ⌜l_t = l_s⌝
-    | PairV v1_t v2_t, PairV v1_s v2_s =>
-        val_rel v1_t v1_s ∧ val_rel v2_t v2_s
-    | InjLV v_t, InjLV v_s =>
-        val_rel v_t v_s
-    | InjRV v_t, InjRV v_s =>
-        val_rel v_t v_s
-    | _,_ => False
-    end.
-  Global Instance val_rel_pers v_t v_s : Persistent (val_rel v_t v_s).
-  Proof.
-    induction v_s as [[] | | | ] in v_t |-*; destruct v_t as [ [] | | | ]; apply _.
-  Qed.
-
-  Lemma val_rel_pair_source v_t v_s1 v_s2 :
-    val_rel v_t (v_s1, v_s2) -∗
-    ∃ v_t1 v_t2, ⌜v_t = PairV v_t1 v_t2⌝ ∗
-      val_rel v_t1 v_s1 ∗
-      val_rel v_t2 v_s2.
-  Proof.
-    simpl. iIntros "H". destruct v_t as [[] | v_t1 v_t2 | |]; simpl; try done.
-    iExists v_t1, v_t2. iDestruct "H" as "[#H1 #H2]". eauto.
-  Qed.
-  Lemma val_rel_injl_source v_t v_s :
-    val_rel v_t (InjLV v_s) -∗ ∃ v_t', ⌜v_t = InjLV v_t'⌝ ∗ val_rel v_t' v_s.
-  Proof. simpl. destruct v_t as [[] | | |]; (try by iIntros "%Hp"); eauto. Qed.
-  Lemma val_rel_injr_source v_t v_s :
-    val_rel v_t (InjRV v_s) -∗ ∃ v_t', ⌜v_t = InjRV v_t'⌝ ∗ val_rel v_t' v_s.
-  Proof. simpl. destruct v_t as [[] | | |]; (try by iIntros "%Hp"); eauto. Qed.
-
-
-  Lemma val_rel_litfn_source v_t fn_s :
-    val_rel v_t (LitV $ LitFn $ fn_s) -∗ ⌜v_t = LitV $ LitFn $ fn_s⌝.
-  Proof. simpl. destruct v_t as [[] | v_t1 v_t2 | |]; iIntros "%Hp"; inversion Hp; subst; done. Qed.
-  Lemma val_rel_litint_source v_t n :
-    val_rel v_t (LitV $ LitInt n) -∗ ⌜v_t = LitV $ LitInt $ n⌝.
-  Proof. simpl. destruct v_t as [[] | v_t1 v_t2 | |]; iIntros "%Hp"; inversion Hp; subst; done. Qed.
-  Lemma val_rel_litbool_source v_t b:
-    val_rel v_t (LitV $ LitBool b) -∗ ⌜v_t = LitV $ LitBool b⌝.
-  Proof. simpl. destruct v_t as [[] | v_t1 v_t2 | |]; iIntros "%Hp"; inversion Hp; subst; done. Qed.
-  Lemma val_rel_litunit_source v_t :
-    val_rel v_t (LitV $ LitUnit) -∗ ⌜v_t = LitV $ LitUnit⌝.
-  Proof. simpl. destruct v_t as [[] | v_t1 v_t2 | |]; iIntros "%Hp"; inversion Hp; subst; done. Qed.
-  Lemma val_rel_litpoison_source v_t :
-    val_rel v_t (LitV $ LitPoison) -∗ ⌜v_t = LitV $ LitPoison⌝.
-  Proof. simpl. destruct v_t as [[] | v_t1 v_t2 | |]; iIntros "%Hp"; inversion Hp; subst; done. Qed.
-  Lemma val_rel_loc_source v_t l_s :
-    val_rel v_t (LitV $ LitLoc l_s) -∗
-    ∃ l_t, ⌜v_t = LitV $ LitLoc l_t⌝ ∗ l_t ↔h l_s.
-  Proof.
-    destruct v_t as [[ | | | | l_t | ] | | | ]; simpl;
-        first [iIntros "%Ht"; congruence | iIntros "#Ht"; eauto].
-  Qed.
-
-  Lemma val_rel_pair_target v_s v_t1 v_t2 :
-    val_rel (v_t1, v_t2) v_s -∗
-    ∃ v_s1 v_s2, ⌜v_s = PairV v_s1 v_s2⌝ ∗
-      val_rel v_t1 v_s1 ∗
-      val_rel v_t2 v_s2.
-  Proof.
-    simpl. iIntros "H". destruct v_s as [[] | v_s1 v_s2 | |]; simpl; try done.
-    iExists v_s1, v_s2. iDestruct "H" as "[#H1 #H2]". eauto.
-  Qed.
-  Lemma val_rel_injl_target v_t v_s :
-    val_rel (InjLV v_t) v_s -∗ ∃ v_s', ⌜v_s = InjLV v_s'⌝ ∗ val_rel v_t v_s'.
-  Proof. simpl. destruct v_s as [[] | | |]; (try by iIntros "%Hp"); eauto. Qed.
-  Lemma val_rel_injr_target v_t v_s :
-    val_rel (InjRV v_t) v_s -∗ ∃ v_s', ⌜v_s = InjRV v_s'⌝ ∗ val_rel v_t v_s'.
-  Proof. simpl. destruct v_s as [[] | | |]; (try by iIntros "%Hp"); eauto. Qed.
-  Lemma val_rel_litfn_target v_s fn_t :
-    val_rel (LitV $ LitFn $ fn_t) v_s -∗ ⌜v_s = LitV $ LitFn $ fn_t⌝.
-  Proof. simpl. destruct v_s as [[] | v_s1 v_s2 | |]; iIntros "%Hp"; inversion Hp; subst; done. Qed.
-  Lemma val_rel_litint_target v_s n :
-    val_rel (LitV $ LitInt n) v_s -∗ ⌜v_s = LitV $ LitInt $ n⌝.
-  Proof. simpl. destruct v_s as [[] | | |]; iIntros "%Hp"; inversion Hp; subst; done. Qed.
-  Lemma val_rel_litbool_target v_s b:
-    val_rel (LitV $ LitBool b) v_s -∗ ⌜v_s = LitV $ LitBool b⌝.
-  Proof. simpl. destruct v_s as [[] | | |]; iIntros "%Hp"; inversion Hp; subst; done. Qed.
-  Lemma val_rel_litunit_target v_s :
-    val_rel (LitV $ LitUnit) v_s -∗ ⌜v_s = LitV $ LitUnit⌝.
-  Proof. simpl. destruct v_s as [[] | | |]; iIntros "%Hp"; inversion Hp; subst; done. Qed.
-  Lemma val_rel_litpoison_target v_s :
-    val_rel (LitV $ LitPoison) v_s -∗ ⌜v_s = LitV $ LitPoison⌝.
-  Proof. simpl. destruct v_s as [[] | | |]; iIntros "%Hp"; inversion Hp; subst; done. Qed.
-  Lemma val_rel_loc_target v_s l_t :
-    val_rel (LitV $ LitLoc l_t) v_s -∗
-    ∃ l_s, ⌜v_s = LitV $ LitLoc l_s⌝ ∗ l_t ↔h l_s.
-  Proof.
-    destruct v_s as [[ | | | | l_s | ] | | | ]; simpl;
-        first [iIntros "%Hs"; congruence | iIntros "#Hs"; eauto].
-  Qed.
-End val_rel.
-Tactic Notation "val_discr_source" constr(H) :=
-  first [iPoseProof (val_rel_litint_source with H) as "->" |
-         iPoseProof (val_rel_litbool_source with H) as "->" |
-         iPoseProof (val_rel_litfn_source with H) as "->" |
-         iPoseProof (val_rel_litunit_source with H) as "->" |
-         iPoseProof (val_rel_litpoison_source with H) as "->" |
-         idtac].
-Tactic Notation "val_discr_target" constr(H) :=
-  first [iPoseProof (val_rel_litint_target with H) as "->" |
-         iPoseProof (val_rel_litbool_target with H) as "->" |
-         iPoseProof (val_rel_litfn_target with H) as "->" |
-         iPoseProof (val_rel_litunit_target with H) as "->" |
-         iPoseProof (val_rel_litpoison_target with H) as "->" |
-         idtac].
-
-Lemma val_rel_func `{heapbijG Σ} v1 v2 v3 : val_rel v1 v2 -∗ val_rel v1 v3 -∗ ⌜v2 = v3⌝.
-Proof.
-  iIntros "Hv1 Hv2". iInduction v2 as [[n2 | b2 | | | l2 | f2 ] | v2_1 v2_2 | v2 | v2] "IH" forall (v1 v3); val_discr_source "Hv1"; val_discr_target "Hv2"; try done.
-  - iPoseProof (val_rel_loc_source with "Hv1") as (?) "(-> & Hl1)".
-    iPoseProof (val_rel_loc_target with "Hv2") as (?) "(-> & Hl2)".
-    by iPoseProof (heap_bij_loc_func with "Hl1 Hl2") as "->".
-  - iPoseProof (val_rel_pair_source with "Hv1") as (??) "(-> & Hv1_1 & Hv1_2)".
-    iPoseProof (val_rel_pair_target with "Hv2") as (??) "(-> & Hv2_1 & Hv2_2)".
-    iPoseProof ("IH" with "Hv1_1 Hv2_1") as "->".
-    by iPoseProof ("IH1" with "Hv1_2 Hv2_2") as "->".
-  - iPoseProof (val_rel_injl_source with "Hv1") as (?) "(-> & Hv1)".
-    iPoseProof (val_rel_injl_target with "Hv2") as (?) "(-> & Hv2)".
-    by iPoseProof ("IH" with "Hv1 Hv2") as "->".
-  - iPoseProof (val_rel_injr_source with "Hv1") as (?) "(-> & Hv1)".
-    iPoseProof (val_rel_injr_target with "Hv2") as (?) "(-> & Hv2)".
-    by iPoseProof ("IH" with "Hv1 Hv2") as "->".
-Qed.
-Lemma val_rel_inj `{heapbijG Σ} v1 v2 v3 : val_rel v2 v1 -∗ val_rel v3 v1 -∗ ⌜v2 = v3⌝.
-Proof.
-  iIntros "Hv1 Hv2". iInduction v2 as [[n2 | b2 | | | l2 | f2 ] | v2_1 v2_2 | v2 | v2] "IH" forall (v1 v3); val_discr_target "Hv1"; val_discr_source "Hv2"; try done.
-  - iPoseProof (val_rel_loc_target with "Hv1") as (?) "(-> & Hl1)".
-    iPoseProof (val_rel_loc_source with "Hv2") as (?) "(-> & Hl2)".
-    by iPoseProof (heap_bij_loc_inj with "Hl1 Hl2") as "->".
-  - iPoseProof (val_rel_pair_target with "Hv1") as (??) "(-> & Hv1_1 & Hv1_2)".
-    iPoseProof (val_rel_pair_source with "Hv2") as (??) "(-> & Hv2_1 & Hv2_2)".
-    iPoseProof ("IH" with "Hv1_1 Hv2_1") as "->".
-    by iPoseProof ("IH1" with "Hv1_2 Hv2_2") as "->".
-  - iPoseProof (val_rel_injl_target with "Hv1") as (?) "(-> & Hv1)".
-    iPoseProof (val_rel_injl_source with "Hv2") as (?) "(-> & Hv2)".
-    by iPoseProof ("IH" with "Hv1 Hv2") as "->".
-  - iPoseProof (val_rel_injr_target with "Hv1") as (?) "(-> & Hv1)".
-    iPoseProof (val_rel_injr_source with "Hv2") as (?) "(-> & Hv2)".
-    by iPoseProof ("IH" with "Hv1 Hv2") as "->".
-Qed.
 
 
 Section definitions.
