theories/simplang/heapbij_refl.v
@@ -70,6 +70,7 @@ Definition ectx_wf : ectx → Prop := Forall ectxi_wf.
 
 Section refl.
   Context `{heapbijG Σ}.
+  Notation log_rel := (log_rel val_rel (const True%I)) (only parsing).
 
   Lemma val_wf_sound v : val_wf v → ⊢ val_rel v v.
   Proof.
@@ -78,313 +79,15 @@ Section refl.
     simpl. destruct Hv as [H1 H2]. iSplit; [by iApply "IH" | by iApply "IH1"].
   Qed.
 
-  Local Lemma call_not_val v1 v2 : language.to_val (Call v1 v2) = None.
-  Proof.
-    rewrite /language.to_val /language.to_class; cbn.
-    destruct to_fname; [destruct to_val | ]; done.
-  Qed.
-
-  Lemma val_rel_val_is_unboxed v_t v_s : val_rel v_t v_s -∗ ⌜val_is_unboxed v_t ↔ val_is_unboxed v_s⌝.
-  Proof.
-    iIntros "Hv".
-    destruct v_s as [[] | | | ]; val_discr_source "Hv"; [ done .. | |done | | |].
-    - by iPoseProof (val_rel_loc_source with "Hv") as (?) "(-> & _)".
-    - by iPoseProof (val_rel_pair_source with "Hv") as (??) "(-> & Hv1 & Hv2)".
-    - iPoseProof (val_rel_injl_source with "Hv") as (?) "(-> & Hv)".
-      destruct v_s as [[] | | | ]; val_discr_source "Hv"; [done.. | | done | | |].
-      + by iPoseProof (val_rel_loc_source with "Hv") as (?) "(-> & _)".
-      + by iPoseProof (val_rel_pair_source with "Hv") as (??) "(-> & Hv1 & Hv2)".
-      + by iPoseProof (val_rel_injl_source with "Hv") as (?) "(-> & Hv)".
-      + by iPoseProof (val_rel_injr_source with "Hv") as (?) "(-> & Hv)".
-    - iPoseProof (val_rel_injr_source with "Hv") as (?) "(-> & Hv)".
-      destruct v_s as [[] | | | ]; val_discr_source "Hv"; [done.. | | done | | |].
-      + by iPoseProof (val_rel_loc_source with "Hv") as (?) "(-> & _)".
-      + by iPoseProof (val_rel_pair_source with "Hv") as (??) "(-> & Hv1 & Hv2)".
-      + by iPoseProof (val_rel_injl_source with "Hv") as (?) "(-> & Hv)".
-      + by iPoseProof (val_rel_injr_source with "Hv") as (?) "(-> & Hv)".
-  Qed.
-
-  (* pull out compatibility lemmas as Iris entailment *)
-
-  Local Tactic Notation "smart_sim_bind" uconstr(ctx_t) uconstr(ctx_s) uconstr(Hp) :=
-    sim_bind ctx_t ctx_s;
-    iApply (sim_wand with Hp).
-
-  Notation log_rel := (log_rel val_rel) (only parsing).
-
-  Lemma log_rel_var x : ⊢ log_rel (Var x) (Var x).
-  Proof.
-    iIntros (? xs) "!# #Hs"; simpl.
-    iDestruct (subst_map_rel_lookup _ x with "Hs") as (v_t v_s Hv) "Hrel"; first set_solver.
-    rewrite !lookup_fmap Hv /=. sim_val. done.
-  Qed.
-
-  Lemma log_rel_let x e1_t e1_s e2_t e2_s :
-    log_rel e1_t e1_s -∗ log_rel e2_t e2_s -∗ log_rel (Let x e1_t e2_t) (Let x e1_s e2_s).
-  Proof.
-    iIntros "#IH1 #IH2" (? xs) "!# #Hs"; simpl.
-    smart_sim_bind (subst_map _ _) (subst_map _ _) "(IH1 [])".
-    { iApply (subst_map_rel_weaken with "[$]"). set_solver. }
-    iIntros (v_t v_s) "#Hv". sim_pures. rewrite !subst'_subst_map.
-    rewrite -(binder_insert_fmap fst (v_t, v_s)).
-    rewrite -(binder_insert_fmap snd (v_t, v_s)).
-    iApply "IH2".
-    iApply (subst_map_rel_insert with "[] Hv").
-    iApply (subst_map_rel_weaken with "[$]").
-    destruct x as [|x]; first set_solver.
-    apply elem_of_subseteq=>x'.
-    destruct (decide (x = x')) as [<-|Hne]; set_solver.
-  Qed.
-
-  Lemma log_rel_call e1_t e1_s e2_t e2_s :
-    log_rel e1_t e1_s -∗ log_rel e2_t e2_s -∗ log_rel (Call e1_t e2_t) (Call e1_s e2_s).
-  Proof.
-    iIntros "#IH1 #IH2" (? xs) "!# #Hs"; simpl.
-    smart_sim_bind (subst_map _ _) (subst_map _ _) "(IH2 [])".
-    { iApply (subst_map_rel_weaken with "[$]"). set_solver. }
-    iIntros (v_t1 v_s1) "#Hv1".
-    smart_sim_bind (subst_map _ _) (subst_map _ _) "(IH1 [])".
-    { iApply (subst_map_rel_weaken with "[$]"). set_solver. }
-    iIntros (v_t2 v_s2) "#Hv2".
-    discr_source; first by apply call_not_val. val_discr_source "Hv2".
-    iApply sim_wand; [ by iApply sim_call|]. iIntros (??) "$".
-  Qed.
-
-  Lemma log_rel_unop e_t e_s o :
-    log_rel e_t e_s -∗ log_rel (UnOp o e_t) (UnOp o e_s).
-  Proof.
-    iIntros "#IH" (? xs) "!# #Hs"; simpl.
-    smart_sim_bind (subst_map _ e_t) (subst_map _ e_s) "(IH [])".
-    { iApply (subst_map_rel_weaken with "[$]"). set_solver. }
-    iIntros (v_t v_s) "#Hv".
-    destruct o; sim_pures; discr_source; val_discr_source "Hv"; by sim_pures; sim_val.
-  Qed.
-
-  Lemma log_rel_binop e1_t e1_s e2_t e2_s o :
-    log_rel e1_t e1_s -∗ log_rel e2_t e2_s -∗ log_rel (BinOp o e1_t e2_t) (BinOp o e1_s e2_s).
-  Proof.
-    iIntros "#IH1 #IH2" (? xs) "!# #Hs"; simpl.
-    smart_sim_bind (subst_map _ e2_t) (subst_map _ e2_s) "(IH2 [])".
-    { iApply (subst_map_rel_weaken with "[$]"). set_solver. }
-    iIntros (v_t2 v_s2) "Hv2".
-    smart_sim_bind (subst_map _ e1_t) (subst_map _ e1_s) "(IH1 [])".
-    { iApply (subst_map_rel_weaken with "[$]"). set_solver. }
-    iIntros (v_t1 v_s1) "Hv1".
-    destruct o; sim_pures; discr_source; val_discr_source "Hv1"; val_discr_source "Hv2"; sim_pures; [sim_val; done .. | | ].
-    - iAssert (⌜vals_compare_safe v_t1 v_t2⌝)%I as "%".
-      { iPoseProof (val_rel_val_is_unboxed with "Hv1") as "%Hv1".
-        iPoseProof (val_rel_val_is_unboxed with "Hv2") as "%Hv2".
-        iPureIntro. by rewrite /vals_compare_safe Hv1 Hv2.
-      }
-      case_bool_decide; subst.
-      * iPoseProof (val_rel_inj with "Hv1 Hv2") as "->".
-        sim_pures; sim_val. case_bool_decide; done.
-      * sim_pures; sim_val. case_bool_decide; subst; last done.
-        by iPoseProof (val_rel_func with "Hv1 Hv2") as "->".
-    - iPoseProof (val_rel_loc_source with "Hv1") as (l_t) "(-> & Hl)".
-      sim_pures. sim_val. iModIntro; cbn.
-      by iApply heap_bij_loc_shift.
-  Qed.
-
-  Lemma log_rel_if e1_t e1_s e2_t e2_s e3_t e3_s :
-    log_rel e1_t e1_s -∗
-    log_rel e2_t e2_s -∗
-    log_rel e3_t e3_s -∗
-    log_rel (If e1_t e2_t e3_t) (If e1_s e2_s e3_s).
-  Proof.
-    iIntros "#IH1 #IH2 #IH3" (? xs) "!# #Hs"; simpl.
-    smart_sim_bind (subst_map _ e1_t) (subst_map _ e1_s) "(IH1 [])".
-    { iApply (subst_map_rel_weaken with "[$]"). set_solver. }
-    iIntros (v_t v_s) "Hv".
-    discr_source. val_discr_source "Hv". destruct x; sim_pures.
-    + iApply "IH2". iApply (subst_map_rel_weaken with "[$]"). set_solver.
-    + iApply "IH3". iApply (subst_map_rel_weaken with "[$]"). set_solver.
-  Qed.
-
-  Lemma log_rel_while e1_t e1_s e2_t e2_s :
-    log_rel e1_t e1_s -∗
-    log_rel e2_t e2_s -∗
-    log_rel (While e1_t e2_t) (While e1_s e2_s).
-  Proof.
-    iIntros "#IH1 #IH2" (? xs) "!# #Hs"; simpl.
-    iApply (sim_while_while _ _ _ _ _ (True)%I with "[//]").
-    iModIntro; iIntros "_".
-    smart_sim_bind (subst_map _ e1_t) (subst_map _ e1_s) "(IH1 [])".
-    { iApply (subst_map_rel_weaken with "[$]"). set_solver. }
-    iIntros (v_t v_s) "Hv".
-    discr_source. val_discr_source "Hv". destruct x; sim_pures.
-    + smart_sim_bind (subst_map _ e2_t) (subst_map _ e2_s) "(IH2 [])".
-      { iApply (subst_map_rel_weaken with "[$]"). set_solver. }
-      iIntros (? ?) "_"; sim_pures. iApply sim_expr_base. iRight. by eauto.
-    + iApply sim_expr_base. iLeft. iExists #(), #(); eauto.
-  Qed.
-
-  Lemma log_rel_pair e1_t e1_s e2_t e2_s :
-    log_rel e1_t e1_s -∗
-    log_rel e2_t e2_s -∗
-    log_rel (Pair e1_t e2_t) (Pair e1_s e2_s).
-  Proof.
-    iIntros "#IH1 #IH2" (? xs) "!# #Hs"; simpl.
-    smart_sim_bind (subst_map _ e2_t) (subst_map _ e2_s) "(IH2 [])".
-    { iApply (subst_map_rel_weaken with "[$]"). set_solver. }
-    iIntros (v_t2 v_s2) "Hv2".
-    smart_sim_bind (subst_map _ e1_t) (subst_map _ e1_s) "(IH1 [])".
-    { iApply (subst_map_rel_weaken with "[$]"). set_solver. }
-    iIntros (v_t1 v_s1) "Hv1".
-    sim_pures; sim_val. iModIntro; iSplit; eauto.
-  Qed.
-
-  Lemma log_rel_fst e_t e_s :
-    log_rel e_t e_s -∗ log_rel (Fst e_t) (Fst e_s).
-  Proof.
-    iIntros "#IH" (? xs) "!# #Hs"; simpl.
-    smart_sim_bind (subst_map _ e_t) (subst_map _ e_s) "(IH [])".
-    { iApply (subst_map_rel_weaken with "[$]"). set_solver. }
-    iIntros (v_t v_s) "Hv".
-    discr_source.
-    iPoseProof (val_rel_pair_source with "Hv") as (??) "(-> & ? & ?)"; by sim_pures; sim_val.
-  Qed.
-  Lemma log_rel_snd e_t e_s :
-    log_rel e_t e_s -∗ log_rel (Snd e_t) (Snd e_s).
-  Proof.
-    iIntros "#IH" (? xs) "!# #Hs"; simpl.
-    smart_sim_bind (subst_map _ e_t) (subst_map _ e_s) "(IH [])".
-    { iApply (subst_map_rel_weaken with "[$]"). set_solver. }
-    iIntros (v_t v_s) "Hv".
-    discr_source.
-    iPoseProof (val_rel_pair_source with "Hv") as (??) "(-> & ? & ?)"; by sim_pures; sim_val.
-  Qed.
-
-  Lemma log_rel_injl e_t e_s :
-    log_rel e_t e_s -∗ log_rel (InjL e_t) (InjL e_s).
-  Proof.
-    iIntros "#IH" (? xs) "!# #Hs"; simpl.
-    smart_sim_bind (subst_map _ e_t) (subst_map _ e_s) "(IH [])".
-    { iApply (subst_map_rel_weaken with "[$]"). set_solver. }
-    iIntros (v_t v_s) "Hv"; by sim_pures; sim_val.
-  Qed.
-  Lemma log_rel_injr e_t e_s :
-    log_rel e_t e_s -∗ log_rel (InjR e_t) (InjR e_s).
-  Proof.
-    iIntros "#IH" (? xs) "!# #Hs"; simpl.
-    smart_sim_bind (subst_map _ e_t) (subst_map _ e_s) "(IH [])".
-    { iApply (subst_map_rel_weaken with "[$]"). set_solver. }
-    iIntros (v_t v_s) "Hv"; by sim_pures; sim_val.
-  Qed.
-
-  Lemma log_rel_match e_t e_s e1_t e1_s e2_t e2_s x1 x2 :
-    log_rel e_t e_s -∗
-    log_rel e1_t e1_s -∗
-    log_rel e2_t e2_s -∗
-    log_rel (Match e_t x1 e1_t x2 e2_t) (Match e_s x1 e1_s x2 e2_s).
-  Proof.
-    iIntros "#IH #IH1 #IH2" (? xs) "!# #Hs"; simpl.
-    smart_sim_bind (subst_map _ e_t) (subst_map _ e_s)  "(IH [])".
-    { iApply (subst_map_rel_weaken with "[$]"). set_solver. }
-    iIntros (v_t v_s) "#Hv".
-    discr_source.
-    + iPoseProof (val_rel_injl_source with "Hv") as (v_t') "(-> & ?)". sim_pures.
-      rewrite !subst'_subst_map.
-      rewrite -(binder_insert_fmap fst (v_t', x)).
-      rewrite -(binder_insert_fmap snd (v_t', x)).
-      iApply "IH1".
-      iApply (subst_map_rel_insert with "[] [//]").
-      iApply (subst_map_rel_weaken with "[$]").
-      destruct x1 as [|x1]; first set_solver.
-      apply elem_of_subseteq=>x'.
-      destruct (decide (x1 = x')) as [<-|Hne]; set_solver.
-    + iPoseProof (val_rel_injr_source with "Hv") as (v_t') "(-> & ?)". sim_pures.
-      rewrite !subst'_subst_map.
-      rewrite -(binder_insert_fmap fst (v_t', x)).
-      rewrite -(binder_insert_fmap snd (v_t', x)).
-      iApply "IH2".
-      iApply (subst_map_rel_insert with "[] [//]").
-      iApply (subst_map_rel_weaken with "[$]").
-      destruct x2 as [|x2]; first set_solver.
-      apply elem_of_subseteq=>x'.
-      destruct (decide (x2 = x')) as [<-|Hne]; set_solver.
-  Qed.
-
-  Lemma log_rel_fork e_t e_s :
-    log_rel e_t e_s -∗ log_rel (Fork e_t) (Fork e_s).
-  Proof.
-    iIntros "#IH" (? xs) "!# #Hs"; simpl.
-    iApply sim_fork; first by sim_pures; sim_val. iIntros (?). sim_pures.
-    iApply (sim_wand with "(IH [])"); eauto.
-  Qed.
-
-  Lemma log_rel_allocN e1_t e1_s e2_t e2_s :
-    log_rel e1_t e1_s -∗ log_rel e2_t e2_s -∗ log_rel (AllocN e1_t e2_t) (AllocN e1_s e2_s).
-  Proof.
-    iIntros "#IH1 #IH2" (? xs) "!# #Hs"; simpl.
-    smart_sim_bind (subst_map _ e2_t) (subst_map _ e2_s) "(IH2 [])".
-    { iApply (subst_map_rel_weaken with "[$]"). set_solver. }
-    iIntros (v_t v_s) "Hv".
-    smart_sim_bind (subst_map _ e1_t) (subst_map _ e1_s) "(IH1 [])".
-    { iApply (subst_map_rel_weaken with "[$]"). set_solver. }
-    iIntros (v_t' v_s') "Hv'".
-    discr_source. val_discr_source "Hv'".
-    target_alloc l_t as "Hl_t" "Ha_t"; first done.
-    source_alloc l_s as "Hl_s" "Ha_s"; first done.
-    iApply (sim_bij_insertN with "Ha_t Ha_s Hl_t Hl_s [Hv]"); [lia | by rewrite replicate_length.. | | ].
-    { iDestruct "Hv" as "#Hv".
-      rewrite big_sepL2_replicate_l; last by rewrite replicate_length.
-      generalize (Z.to_nat x) => n.
-      iInduction n as [] "IHn"; cbn; first done. iFrame "Hv IHn".
-    }
-    iIntros "Hv". sim_pures. sim_val. done.
-  Qed.
-
-  Lemma log_rel_freeN e1_t e1_s e2_t e2_s :
-    log_rel e1_t e1_s -∗ log_rel e2_t e2_s -∗ log_rel (FreeN e1_t e2_t) (FreeN e1_s e2_s).
-  Proof.
-    iIntros "#IH1 #IH2" (? xs) "!# #Hs"; simpl.
-    smart_sim_bind (subst_map _ _) (subst_map _ _) "(IH2 [])".
-    { iApply (subst_map_rel_weaken with "[$]"). set_solver. }
-    iIntros (v_t v_s) "Hv".
-    smart_sim_bind (subst_map _ _) (subst_map _ _) "(IH1 [])".
-    { iApply (subst_map_rel_weaken with "[$]"). set_solver. }
-    iIntros (v_t' v_s') "Hv'".
-    discr_source. iPoseProof (val_rel_loc_source with "Hv") as (l_t) "(-> & Hrel)".
-    iPoseProof (val_rel_litint_source with "Hv'") as "->".
-    by sim_free; sim_val.
-  Qed.
-
-  Lemma log_rel_load o e_t e_s :
-    log_rel e_t e_s -∗ log_rel (Load o e_t) (Load o e_s).
-  Proof.
-    iIntros "#IH" (? xs) "!# #Hs"; simpl.
-    smart_sim_bind (subst_map _ _) (subst_map _ _) "(IH [])".
-    { iApply (subst_map_rel_weaken with "[$]"). set_solver. }
-    iIntros (v_t v_s) "Hv". discr_source. iPoseProof (val_rel_loc_source with "Hv") as (l_t) "(-> & Hrel)".
-    by sim_load v_t v_s as "Hv"; sim_val.
-  Qed.
-
-  Lemma log_rel_store o e1_t e1_s e2_t e2_s :
-    log_rel e1_t e1_s -∗ log_rel e2_t e2_s -∗ log_rel (Store o e1_t e2_t) (Store o e1_s e2_s).
-  Proof.
-    iIntros "#IH1 #IH2" (? xs) "!# #Hs"; simpl.
-    smart_sim_bind (subst_map _ _) (subst_map _ _) "(IH2 [])".
-    { iApply (subst_map_rel_weaken with "[$]"). set_solver. }
-    iIntros (v_t v_s) "Hv". (* FIXME: fix printing *)
-    smart_sim_bind (subst_map _ _) (subst_map _ _) "(IH1 [])".
-    { iApply (subst_map_rel_weaken with "[$]"). set_solver. }
-    iIntros (v_t' v_s') "Hv'".
-    discr_source. iPoseProof (val_rel_loc_source with "Hv'") as (l_t) "(-> & Hrel)".
-    by sim_store; [done | sim_val].
-  Qed.
-
-  Lemma log_rel_val v_t v_s :
-    val_rel v_t v_s -∗ log_rel (Val v_t) (Val v_s).
-  Proof. iIntros "#Hv" (? xs) "!# #Hs"; simpl. by sim_val. Qed.
-
   Theorem expr_wf_sound e : expr_wf e → ⊢ log_rel e e.
   Proof.
-    intros Hwf. iInduction e as [ ] "IH" forall (Hwf); iIntros (? xs) "!# #Hs"; simpl.
-    - (* Val *) iApply log_rel_val; [by iApply val_wf_sound | done].
+    intros Hwf. iInduction e as [ ] "IH" forall (Hwf).
+    - (* Val *) iApply log_rel_val. by iApply val_wf_sound.
     - (* Var *) by iApply log_rel_var.
     - (* Let *) destruct Hwf as [Hwf1 Hwf2]. by iApply (log_rel_let with "(IH [//]) (IH1 [//])").
-    - (* Call *) destruct Hwf as [Hwf1 Hwf2]. by iApply (log_rel_call with "(IH [//]) (IH1 [//])").
+    - (* Call *)
+      destruct Hwf as [Hwf1 Hwf2]. iApply (log_rel_call with "(IH [//]) (IH1 [//])").
+      iIntros (???). by rewrite left_id.
     - (* UnOp *) by iApply (log_rel_unop with "(IH [//])").
     - (* BinOp *) destruct Hwf as [Hwf1 Hwf2]. by iApply (log_rel_binop with "(IH [//]) (IH1 [//])").
     - (* If *) destruct Hwf as (Hwf1 & Hwf2 & Hwf3). by iApply (log_rel_if with "(IH [//]) (IH1 [//]) (IH2 [//])").
@@ -396,11 +99,32 @@ Section refl.
     - (* InjR *) by iApply (log_rel_injr with "(IH [//])").
     - (* Match *) destruct Hwf as (Hwf1 & Hwf2 & Hwf3).
       by iApply (log_rel_match with "(IH [//]) (IH1 [//]) (IH2 [//])").
-    - (* Fork *) by iApply (log_rel_fork with "(IH [//])").
-    - (* AllocN *) destruct Hwf as (Hwf1 & Hwf2). by iApply (log_rel_allocN with "(IH [//]) (IH1 [//])").
-    - (* FreeN *) destruct Hwf as (Hwf1 & Hwf2). by iApply (log_rel_freeN with "(IH [//]) (IH1 [//])").
-    - (* Load *) by iApply (log_rel_load with "(IH [//])").
-    - (* Store *) destruct Hwf as (Hwf1 & Hwf2). by iApply (log_rel_store with "(IH [//]) (IH1 [//])").
+    - (* Fork *)
+      iApply (log_rel_fork with "(IH [//])").
+      iIntros (?????) "Hsim Hfork". iApply (sim_fork with "(Hsim [//])").
+      iIntros (?). iApply (sim_wand with "[Hfork]"). { by iApply "Hfork". }
+      iIntros (??) "[_ $]".
+    - (* AllocN *)
+      destruct Hwf as (Hwf1 & Hwf2). iApply (log_rel_allocN with "(IH [//]) (IH1 [//])").
+      iIntros (???????) "Hv Hcont".
+      target_alloc l_t as "Hl_t" "Ha_t"; first done.
+      source_alloc l_s as "Hl_s" "Ha_s"; first done.
+      iApply (sim_bij_insertN with "Ha_t Ha_s Hl_t Hl_s [Hv]"); [lia | by rewrite replicate_length.. | | ].
+      { iDestruct "Hv" as "#Hv".
+        rewrite big_sepL2_replicate_l; last by rewrite replicate_length.
+        generalize (Z.to_nat n) => n'.
+        iInduction n' as [] "IHn"; cbn; first done. iFrame "Hv IHn".
+      }
+      by iApply "Hcont".
+    - (* FreeN *)
+      destruct Hwf as (Hwf1 & Hwf2). iApply (log_rel_freeN with "(IH [//]) (IH1 [//])").
+      iIntros (???????) "Hv Hcont". sim_free. by iApply "Hcont".
+    - (* Load *)
+      iApply (log_rel_load with "(IH [//])").
+      iIntros (?????) "Hv Hcont". iApply (sim_bij_load with "Hv"). iIntros (??). by iApply "Hcont".
+    - (* Store *)
+      destruct Hwf as (Hwf1 & Hwf2). iApply (log_rel_store with "(IH [//]) (IH1 [//])").
+      iIntros (???????) "Hl Hv Hcont". iApply (sim_bij_store with "Hl Hv"). by iApply "Hcont".
     - done.
     - done.
   Qed.
